coq/Alt_sem.v
@@ -1,0 +1,163 @@
+(** * An Alternate Abstract Execution Semantics
+
+    This section provides a semantics for produres using traces and
+    unique lists instead of execution.  See [sem'].  Some people might
+    find this definition more intuitive. *)
+
+Require Import FunInd Program Arith Lia.
+Require Import Monad Proc Alg Sem Sem_tactics.
+Import List.ListNotations.
+Open Scope list_scope.
+
+(** Extract the inputs from a runtime environment. *)
+
+Definition get_ins (ev: env) (ds: list decl): list alg :=
+  map snd (skipn (length ev - length ds) ev).
+
+Functional Scheme mk_env_ind :=
+  Induction for mk_env Sort Prop.
+
+Lemma ins_inputs_length:
+  forall inputs ds,
+    ins_inputs ds inputs ->
+    length (mk_env ds inputs) = length ds.
+Proof.
+  intros.
+  functional induction (mk_env ds inputs); auto.
+  - inv H.
+  - inv H; simpl.
+    apply IHe in H6.
+    rewrite H6; auto.
+Qed.
+
+Lemma get_ins_inputs:
+  forall inputs ds ev,
+    ins_inputs ds inputs ->
+    get_ins (ev ++ mk_env ds inputs) ds = inputs.
+Proof.
+  intros.
+  unfold get_ins.
+  rewrite skipn_app.
+  rewrite app_length.
+  rewrite ins_inputs_length; auto.
+  assert (G: length ev +
+             length ds -
+             length ds = length ev).
+  lia.
+  rewrite G.
+  rewrite skipn_all.
+  rewrite app_nil_l.
+  rewrite minus_diag; simpl.
+  clear G.
+  induction H; simpl; auto.
+  rewrite IHins_inputs; auto.
+Qed.
+
+(** Function [get_ins] gets the correct inputs. *)
+
+Lemma sem_implies_inputs:
+  forall (p: proc) (ev: env) (ex: role),
+    sem p ev ex ->
+    inputs ex = get_ins ev (ins p).
+Proof.
+  intros.
+  destruct H.
+  apply stmt_list_sem_env_extends in H0.
+  destruct H0 as [ev']; subst.
+  eapply get_ins_inputs in H; eauto.
+Qed.
+
+(** Get the outputs from a runtime environment and some statements. *)
+
+Fixpoint get_outs (ev: env) (stmts: list stmt): option (list alg) :=
+  match stmts with
+  | [] => None
+  | [Return vs] => map_m (flip lookup ev) vs
+  | stmt :: stmts => get_outs ev stmts
+  end.
+
+Functional Scheme get_outs_ind :=
+  Induction for get_outs Sort Prop.
+
+(** Function [get_outs] gets the correct outputs. *)
+
+Lemma stmt_list_sem_implies_outputs:
+  forall ev tr us outs stmts ev',
+    stmt_list_sem ev tr us outs stmts ev' [] [] ->
+    get_outs ev' stmts = Some outs.
+Proof.
+  intros.
+  revert H.
+  revert ev.
+  revert tr.
+  revert us.
+  functional induction (get_outs ev' stmts); intros.
+  - inv H.
+  - inv H; auto.
+    inv H6.
+  - inv H.
+    inv H6.
+  - inv H.
+    apply IHo in H10; auto.
+  - inv H.
+    apply IHo in H10; auto.
+  - inv H.
+    apply IHo in H10; auto.
+Qed.
+
+Lemma sem_implies_outputs:
+  forall (p: proc) (ev: env) (ex: role),
+    sem p ev ex ->
+    get_outs ev (body p) = Some (outputs ex).
+Proof.
+  intros.
+  unfold sem in H.
+  destruct H.
+  clear H.
+  apply stmt_list_sem_implies_outputs in H0; auto.
+Qed.
+
+(** The alternate abstract execution semantics for procedures *)
+
+Definition sem' (p: proc) (ev: env) (tr: list evt) (us: list alg): Prop :=
+  let inputs := get_ins ev (ins p) in
+  let ev_in := mk_env (ins p) inputs in
+  ins_inputs (ins p) inputs /\
+  exists outs,
+    get_outs ev (body p) = Some outs /\
+    stmt_list_sem ev_in tr us outs (body p) ev [] [].
+
+Lemma sem_implies_sem':
+  forall (p: proc) (ev: env) (ex: role),
+    sem p ev ex ->
+    sem' p ev (trace ex) (uniqs ex).
+Proof.
+  intros.
+  pose proof H as G.
+  apply sem_implies_inputs in G.
+  pose proof H as F.
+  apply sem_implies_outputs in F.
+  unfold sem in H.
+  destruct H as [E H].
+  rewrite G in E.
+  rewrite G in H.
+  unfold sem'.
+  split; auto.
+  exists (outputs ex); split; auto.
+Qed.
+
+Lemma sem'_implies_sem:
+  forall (p: proc) (ev: env) (tr: list evt) (us: list alg),
+    sem' p ev tr us ->
+    exists outs,
+      get_outs ev (body p) = Some outs /\
+      let ins := get_ins ev (ins p) in
+      sem p ev (mkRole tr us ins outs).
+Proof.
+  intros.
+  unfold sem' in H.
+  destruct H.
+  destruct H0 as [outs].
+  exists outs.
+  unfold sem; simpl; intuition.
+Qed.
